Introduce inductive definition of reborrow in another file (#5)

Rustv/BorrowStack.thy
@@ -701,174 +701,6 @@ next
     using hd_dropWhile_stack assms writable_in_collect_tags by simp
 qed
 
-inductive reborrow'
-  :: "ref_kind \<Rightarrow> tag \<Rightarrow> tag \<Rightarrow> (ref_kind * tag set) stack \<Rightarrow> (ref_kind * tag set) stack \<Rightarrow> bool" where
-  DerivUniqueUnique:
-    "reborrow' Unique deriv orig
-      ((Unique, {orig}) # tail)
-      ((Unique, {deriv}) # (Unique, {orig}) # tail)" |
-  DerivUniqueSRW:
-    "reborrow' SharedReadWrite deriv orig
-      ((Unique, {orig}) # tail)
-      ((SharedReadWrite, {deriv}) # (Unique, {orig}) # tail)" |
-  DerivUniqueSRO:
-    "reborrow' SharedReadOnly deriv orig
-      ((Unique, {orig}) # tail)
-      ((SharedReadOnly, {deriv}) # (Unique, {orig}) # tail)" |
-  DerivSRWUnique:
-    "orig \<in> ts
-     \<Longrightarrow> reborrow' Unique deriv orig
-      ((SharedReadWrite, ts) # tail)
-      ((Unique, {deriv}) # (SharedReadWrite, ts) # tail)" |
-  DerivSRWSRW:
-    "orig \<in> ts
-     \<Longrightarrow> reborrow' SharedReadWrite deriv orig
-      ((SharedReadWrite, ts) # tail)
-      ((SharedReadWrite, insert deriv ts) # tail)" |
-  DerivSRWSRO:
-    "orig \<in> ts
-     \<Longrightarrow> reborrow' SharedReadOnly deriv orig
-      ((SharedReadWrite, ts) # tail)
-      ((SharedReadOnly, {deriv}) # (SharedReadWrite, ts) # tail)" |
-  DerivSROSRO:
-    "orig \<in> ts
-     \<Longrightarrow> reborrow' SharedReadOnly deriv orig
-      ((SharedReadOnly, ts) # tail)
-      ((SharedReadOnly, insert deriv ts) # tail)" |
-  DerivPop:
-    "\<lbrakk>reborrow' k deriv orig tail stack; orig \<notin> snd entry\<rbrakk>
-    \<Longrightarrow> reborrow' k deriv orig (entry # tail) stack"
-
-lemma reborrow'_nonempty_src:
-  "reborrow' k deriv orig stack stack' \<Longrightarrow> stack \<noteq> []"
-  using reborrow'.simps by blast
-
-lemma ex_reborrow'_writable:
-  assumes
-    "wf_reborrow stack"
-    "writable orig stack"
-  shows "\<exists>stack'. reborrow' k deriv orig stack stack'"
-using assms proof (induction rule: wf_reborrow_induct')
-  case (Root t)
-  then show ?case
-    by (metis (full_types) DerivUniqueSRO DerivUniqueSRW DerivUniqueUnique empty_iff insert_iff
-        ref_kind.exhaust writable.simps(1) writable.simps(2))
-next
-  case (UniqueUnique t t' tail)
-  then show ?case
-    by (metis (full_types) DerivPop DerivUniqueSRO DerivUniqueSRW DerivUniqueUnique
-        ref_kind.exhaust singletonD snd_conv writable.simps(2))
-next
-  case (UniqueSRW t ts' tail)
-  then show ?case
-    by (metis (full_types) DerivPop DerivSRWSRO DerivSRWSRW DerivSRWUnique
-        ref_kind.exhaust snd_eqD writable.simps(2))
-next
-  case (UniqueSRO t ts' tail)
-  then show ?case
-    by (metis DerivPop ref_kind.distinct(3) ref_kind.distinct(5) snd_conv writable.simps(2))
-next
-  case (SRWUnique ts t' tail)
-  then show ?case
-    by (metis (full_types) DerivPop DerivUniqueSRO DerivUniqueSRW DerivUniqueUnique
-        ref_kind.exhaust singletonD snd_eqD writable.simps(2))
-next
-  case (SRWSRO ts ts' tail)
-  then show ?case
-    by (metis DerivPop ref_kind.distinct(3) ref_kind.distinct(5) sndI writable.simps(2))
-qed
-
-lemma ex_reborrow'_readable:
-  assumes
-    "wf_reborrow stack"
-    "readable orig stack"
-    "k = SharedReadOnly"
-  shows "\<exists>stack'. reborrow' k deriv orig stack stack'"
-using assms proof (induction rule: wf_reborrow_induct')
-  case (Root t)
-  then show ?case using DerivUniqueSRO by auto
-next
-  case (UniqueUnique t t' tail)
-  then show ?case
-  proof (cases "t' = orig")
-    case True
-    then show ?thesis using UniqueUnique DerivUniqueSRO by auto
-  next
-    case False
-    then show ?thesis
-    proof -
-      obtain stack' where
-        "reborrow' k deriv orig ((Unique, {t}) # tail) stack'"
-        using UniqueUnique False by auto
-      then show ?thesis using False DerivPop by force
-    qed
-  qed
-next
-  case (UniqueSRW t ts' tail)
-  then show ?case
-  proof (cases "orig \<in> ts'")
-    case True
-    then show ?thesis using UniqueSRW DerivSRWSRO by blast
-  next
-    case False
-    then show ?thesis
-    proof -
-      obtain stack' where
-        "reborrow' k deriv orig ((Unique, {t}) # tail) stack'"
-        using UniqueSRW False by auto
-      then show ?thesis using False DerivPop by force
-    qed
-  qed
-next
-  case (UniqueSRO t ts' tail)
-  then show ?case
-  proof (cases "orig \<in> ts'")
-    case True
-    then show ?thesis using UniqueSRO DerivSROSRO by blast
-  next
-    case False
-    then show ?thesis
-    proof -
-      obtain stack' where
-        "reborrow' k deriv orig ((Unique, {t}) # tail) stack'"
-        using UniqueSRO False by auto
-      then show ?thesis using False DerivPop by force
-    qed
-  qed
-next
-  case (SRWUnique ts t' tail)
-  then show ?case
-  proof (cases "t' = orig")
-    case True
-    then show ?thesis using SRWUnique DerivUniqueSRO by auto
-  next
-    case False
-    then show ?thesis
-    proof -
-      obtain stack' where
-        "reborrow' k deriv orig ((SharedReadWrite, ts) # tail) stack'"
-        using SRWUnique False by auto
-      then show ?thesis using False DerivPop by force
-    qed
-  qed
-next
-  case (SRWSRO ts ts' tail)
-  then show ?case
-  proof (cases "orig \<in> ts'")
-    case True
-    then show ?thesis using SRWSRO DerivSROSRO by blast
-  next
-    case False
-    then show ?thesis
-    proof -
-      obtain stack' where
-        "reborrow' k deriv orig ((SharedReadWrite, ts) # tail) stack'"
-        using SRWSRO False by auto
-      then show ?thesis using False DerivPop by force
-    qed
-  qed
-qed
-
 (* computational definition of reborrow *)
 fun reborrow :: "ref_kind \<Rightarrow> tag \<Rightarrow> (ref_kind * tag set) stack \<Rightarrow> (ref_kind * tag set) stack"
   where
@@ -898,42 +730,11 @@ fun reborrow_comp
   "reborrow_comp k child parent stack =
     reborrow k child (pop_tags parent stack)"
 
-fun reborrow_ind
-  :: "ref_kind \<Rightarrow> tag \<Rightarrow> tag \<Rightarrow> (ref_kind * tag set) stack \<Rightarrow> (ref_kind * tag set) stack" where
-  "reborrow_ind k deriv orig stack = (THE stack'. reborrow' k deriv orig stack stack')"
-
-lemma reborrow_by_comp[simp, intro]:
-  "reborrow' k deriv orig stack stack' \<Longrightarrow> reborrow_comp k deriv orig stack = stack'"
-proof (induction rule: reborrow'.induct)
-qed simp_all
-
-lemma reborrow_unique:
-  assumes
-    "reborrow' k deriv orig stack stack'"
-    "reborrow' k deriv orig stack stack''"
-  shows "stack' = stack''"
-  using assms(1) assms(2) reborrow_by_comp by blast
-
 lemma reborrow_comp_pop:
   assumes "orig \<notin> snd entry"
   shows "reborrow_comp k deriv orig (entry # stack) = reborrow_comp k deriv orig stack"
 using assms proof (induction stack, auto)
 qed
-
-lemma the_reborrow'_writable:
-  assumes
-    "wf_reborrow stack"
-    "writable orig stack"
-  shows "\<exists>!stack'. reborrow' k deriv orig stack stack'"
-  using assms ex_reborrow'_writable reborrow_unique by auto
-
-lemma the_reborrow'_readable:
-  assumes
-    "wf_reborrow stack"
-    "readable orig stack"
-    "k = SharedReadOnly"
-  shows "\<exists>!stack'. reborrow' k deriv orig stack stack'"
-  using assms ex_reborrow'_readable reborrow_unique by fastforce
 
 lemma reborrow_hd:
   assumes
@@ -942,12 +743,6 @@ lemma reborrow_hd:
   shows "k = fst (hd stack') \<and> t \<in> snd (hd stack')"
 using assms proof (cases rule: reborrow.elims)
 qed auto
-
-lemma reborrow'_hd:
-  assumes "reborrow' k deriv orig stack stack'"
-  shows "k = fst (hd stack') \<and> deriv \<in> snd (hd stack')"
-using assms proof (induction rule: reborrow'.induct, auto)
-qed
 
 fun_cases reborrow_elims_Unique[case_names _ UniqueUnique UniqueSRW]:
   "reborrow Unique t stack = (Unique, ts) # stack'"
@@ -1071,17 +866,6 @@ next
   then show ?thesis using assms wf_reborrow_reborrow_SRO by simp
 qed
 
-lemma wf_reborrow_reborrow':
-  assumes
-    "reborrow' k deriv orig stack stack'"
-    "wf_reborrow stack"
-    "deriv \<notin> collect_tags stack"
-  shows "wf_reborrow stack'"
-using assms proof (induction)
-  case (DerivPop k deriv orig tail stack entry)
-  then show ?case using reborrow'_nonempty_src wf_reborrow_pop' by auto
-qed (auto simp add: ReborrowSRWSRW ReborrowSROSRO)
-
 lemma collect_tags_reborrow_subset:
   assumes "reborrow k t stack = stack'"
   shows "collect_tags stack' \<subseteq> {t} \<union> collect_tags stack"
@@ -1095,14 +879,6 @@ lemma stack_finite_reborrow:
   shows "stack_finite stack'"
 using assms collect_tags_reborrow_subset stack_finite_finite_collect_tags
   by (meson collect_tags_stack_finite finite.emptyI finite.insertI finite_Un finite_subset)
-
-lemma stack_finite_reborrow':
-  assumes
-    "reborrow' k deriv orig stack stack'"
-    "stack_finite stack"
-  shows "stack_finite stack'"
-using assms proof (induction, auto)
-qed
 
 lemma notin_pop_tags:
   assumes "pop_tags t stack = stack'"
@@ -1185,12 +961,6 @@ proof -
         using assms calculation p q ReborrowSRWSRO by simp
     qed
   qed
-qed
-
-lemma reborrow'_subset:
-  assumes "reborrow' k deriv orig stack stack'"
-  shows "collect_tags stack' \<subseteq> {deriv} \<union> collect_tags stack"
-using assms proof (induction, auto)
 qed
 
 lemma reborrow_comp_subset:
@@ -1330,44 +1100,6 @@ lemma writable_reborrow_comp_derived:
     "k = Unique \<or> k = SharedReadWrite"
   shows "writable t' stack'"
 using assms proof (cases rule: decomp_reborrow_comp_writable_elims)
-qed auto
-
-lemma writable_reborrow:
-  assumes
-    "reborrow' k deriv orig stack stack'"
-    "wf_reborrow stack"
-    "writable orig stack"
-    "deriv \<notin> collect_tags stack"
-  shows "writable orig stack'"
-using assms proof (induction)
-  case (DerivPop k deriv orig tail stack entry)
-  show ?case
-  proof (rule DerivPop.IH)
-    show "wf_reborrow tail" using DerivPop wf_reborrow_pop' reborrow'_nonempty_src by simp
-  next
-    show "writable orig tail" using DerivPop writable_tl by fastforce
-  next
-    show "deriv \<notin> collect_tags tail" using DerivPop.prems by simp
-  qed
-qed auto
-
-lemma writable_reborrow_derived:
-  assumes
-    "reborrow' k deriv orig stack stack'"
-    "writable orig stack"
-    "wf_reborrow stack"
-    "k = Unique \<or> k = SharedReadWrite"
-  shows "writable deriv stack'"
-using assms proof (induction)
-  case (DerivPop k deriv orig tail stack entry)
-  show ?case
-  proof (rule DerivPop.IH)
-    show "wf_reborrow tail" using DerivPop wf_reborrow_pop' reborrow'_nonempty_src by simp
-  next
-    show "writable orig tail" using DerivPop writable_tl by fastforce
-  next
-    show "k = Unique \<or> k = SharedReadWrite" using DerivPop.prems by simp
-  qed
 qed auto
 
 end
