Rustv/ReborrowInd.thy
@@ -1,0 +1,340 @@
+theory ReborrowInd
+  imports BorrowStack
+begin
+
+inductive reborrow'
+  :: "ref_kind \<Rightarrow> tag \<Rightarrow> tag \<Rightarrow> (ref_kind * tag set) stack \<Rightarrow> (ref_kind * tag set) stack \<Rightarrow> bool" where
+  DerivUniqueUnique:
+    "reborrow' Unique deriv orig
+      ((Unique, {orig}) # tail)
+      ((Unique, {deriv}) # (Unique, {orig}) # tail)" |
+  DerivUniqueSRW:
+    "reborrow' SharedReadWrite deriv orig
+      ((Unique, {orig}) # tail)
+      ((SharedReadWrite, {deriv}) # (Unique, {orig}) # tail)" |
+  DerivUniqueSRO:
+    "reborrow' SharedReadOnly deriv orig
+      ((Unique, {orig}) # tail)
+      ((SharedReadOnly, {deriv}) # (Unique, {orig}) # tail)" |
+  DerivSRWUnique:
+    "orig \<in> ts
+     \<Longrightarrow> reborrow' Unique deriv orig
+      ((SharedReadWrite, ts) # tail)
+      ((Unique, {deriv}) # (SharedReadWrite, ts) # tail)" |
+  DerivSRWSRW:
+    "orig \<in> ts
+     \<Longrightarrow> reborrow' SharedReadWrite deriv orig
+      ((SharedReadWrite, ts) # tail)
+      ((SharedReadWrite, insert deriv ts) # tail)" |
+  DerivSRWSRO:
+    "orig \<in> ts
+     \<Longrightarrow> reborrow' SharedReadOnly deriv orig
+      ((SharedReadWrite, ts) # tail)
+      ((SharedReadOnly, {deriv}) # (SharedReadWrite, ts) # tail)" |
+  DerivSROSRO:
+    "orig \<in> ts
+     \<Longrightarrow> reborrow' SharedReadOnly deriv orig
+      ((SharedReadOnly, ts) # tail)
+      ((SharedReadOnly, insert deriv ts) # tail)" |
+  DerivPop:
+    "\<lbrakk>reborrow' k deriv orig tail stack; orig \<notin> snd entry\<rbrakk>
+    \<Longrightarrow> reborrow' k deriv orig (entry # tail) stack"
+
+lemma reborrow'_nonempty_src:
+  "reborrow' k deriv orig stack stack' \<Longrightarrow> stack \<noteq> []"
+  using reborrow'.simps by blast
+
+lemma ex_reborrow'_writable:
+  assumes
+    "wf_reborrow stack"
+    "writable orig stack"
+  shows "\<exists>stack'. reborrow' k deriv orig stack stack'"
+using assms proof (induction rule: wf_reborrow_induct')
+  case (Root t)
+  then show ?case
+    by (metis (full_types) DerivUniqueSRO DerivUniqueSRW DerivUniqueUnique empty_iff insert_iff
+        ref_kind.exhaust writable.simps(1) writable.simps(2))
+next
+  case (UniqueUnique t t' tail)
+  then show ?case
+    by (metis (full_types) DerivPop DerivUniqueSRO DerivUniqueSRW DerivUniqueUnique
+        ref_kind.exhaust singletonD snd_conv writable.simps(2))
+next
+  case (UniqueSRW t ts' tail)
+  then show ?case
+    by (metis (full_types) DerivPop DerivSRWSRO DerivSRWSRW DerivSRWUnique
+        ref_kind.exhaust snd_eqD writable.simps(2))
+next
+  case (UniqueSRO t ts' tail)
+  then show ?case
+    by (metis DerivPop ref_kind.distinct(3) ref_kind.distinct(5) snd_conv writable.simps(2))
+next
+  case (SRWUnique ts t' tail)
+  then show ?case
+    by (metis (full_types) DerivPop DerivUniqueSRO DerivUniqueSRW DerivUniqueUnique
+        ref_kind.exhaust singletonD snd_eqD writable.simps(2))
+next
+  case (SRWSRO ts ts' tail)
+  then show ?case
+    by (metis DerivPop ref_kind.distinct(3) ref_kind.distinct(5) sndI writable.simps(2))
+qed
+
+lemma ex_reborrow'_readable:
+  assumes
+    "wf_reborrow stack"
+    "readable orig stack"
+    "k = SharedReadOnly"
+  shows "\<exists>stack'. reborrow' k deriv orig stack stack'"
+using assms proof (induction rule: wf_reborrow_induct')
+  case (Root t)
+  then show ?case using DerivUniqueSRO by auto
+next
+  case (UniqueUnique t t' tail)
+  then show ?case
+  proof (cases "t' = orig")
+    case True
+    then show ?thesis using UniqueUnique DerivUniqueSRO by auto
+  next
+    case False
+    then show ?thesis
+    proof -
+      obtain stack' where
+        "reborrow' k deriv orig ((Unique, {t}) # tail) stack'"
+        using UniqueUnique False by auto
+      then show ?thesis using False DerivPop by force
+    qed
+  qed
+next
+  case (UniqueSRW t ts' tail)
+  then show ?case
+  proof (cases "orig \<in> ts'")
+    case True
+    then show ?thesis using UniqueSRW DerivSRWSRO by blast
+  next
+    case False
+    then show ?thesis
+    proof -
+      obtain stack' where
+        "reborrow' k deriv orig ((Unique, {t}) # tail) stack'"
+        using UniqueSRW False by auto
+      then show ?thesis using False DerivPop by force
+    qed
+  qed
+next
+  case (UniqueSRO t ts' tail)
+  then show ?case
+  proof (cases "orig \<in> ts'")
+    case True
+    then show ?thesis using UniqueSRO DerivSROSRO by blast
+  next
+    case False
+    then show ?thesis
+    proof -
+      obtain stack' where
+        "reborrow' k deriv orig ((Unique, {t}) # tail) stack'"
+        using UniqueSRO False by auto
+      then show ?thesis using False DerivPop by force
+    qed
+  qed
+next
+  case (SRWUnique ts t' tail)
+  then show ?case
+  proof (cases "t' = orig")
+    case True
+    then show ?thesis using SRWUnique DerivUniqueSRO by auto
+  next
+    case False
+    then show ?thesis
+    proof -
+      obtain stack' where
+        "reborrow' k deriv orig ((SharedReadWrite, ts) # tail) stack'"
+        using SRWUnique False by auto
+      then show ?thesis using False DerivPop by force
+    qed
+  qed
+next
+  case (SRWSRO ts ts' tail)
+  then show ?case
+  proof (cases "orig \<in> ts'")
+    case True
+    then show ?thesis using SRWSRO DerivSROSRO by blast
+  next
+    case False
+    then show ?thesis
+    proof -
+      obtain stack' where
+        "reborrow' k deriv orig ((SharedReadWrite, ts) # tail) stack'"
+        using SRWSRO False by auto
+      then show ?thesis using False DerivPop by force
+    qed
+  qed
+qed
+
+fun reborrow_ind
+  :: "ref_kind \<Rightarrow> tag \<Rightarrow> tag \<Rightarrow> (ref_kind * tag set) stack \<Rightarrow> (ref_kind * tag set) stack" where
+  "reborrow_ind k deriv orig stack = (THE stack'. reborrow' k deriv orig stack stack')"
+
+lemma reborrow_by_comp[simp, intro]:
+  "reborrow' k deriv orig stack stack' \<Longrightarrow> reborrow_comp k deriv orig stack = stack'"
+proof (induction rule: reborrow'.induct)
+qed simp_all
+
+lemma the_reborrow_by_comp[simp, intro]:
+  assumes "reborrow' k deriv orig stack (reborrow_comp k deriv orig stack)"
+  shows "(THE stack'. reborrow' k deriv orig stack stack') = reborrow_comp k deriv orig stack"
+  using assms reborrow_by_comp by blast
+
+lemma the_reborrow_by_comp'[simp, intro]:
+  assumes "reborrow' k deriv orig stack (reborrow_comp k deriv orig stack)"
+  shows "The (reborrow' k deriv orig stack) = reborrow_comp k deriv orig stack"
+  using assms the_reborrow_by_comp by simp
+
+lemma reborrow_unique:
+  assumes
+    "reborrow' k deriv orig stack stack'"
+    "reborrow' k deriv orig stack stack''"
+  shows "stack' = stack''"
+  using assms(1) assms(2) reborrow_by_comp by blast
+
+lemma ex1_reborrow'_writable:
+  assumes
+    "wf_reborrow stack"
+    "writable orig stack"
+  shows "\<exists>!stack'. reborrow' k deriv orig stack stack'"
+proof -
+  obtain stack' where
+    *: "reborrow' k deriv orig stack stack'"
+    using assms ex_reborrow'_writable by blast
+  moreover have "\<forall>stack''. reborrow' k deriv orig stack stack'' \<longrightarrow> stack'' = stack'"
+    using reborrow_unique * by auto
+  ultimately show ?thesis by blast
+qed
+
+lemma ex1_reborrow'_readable:
+  assumes
+    "wf_reborrow stack"
+    "readable orig stack"
+    "k = SharedReadOnly"
+  shows "\<exists>!stack'. reborrow' k deriv orig stack stack'"
+proof -
+  obtain stack' where
+    *: "reborrow' k deriv orig stack stack'"
+    using assms ex_reborrow'_readable by blast
+  moreover have "\<forall>stack''. reborrow' k deriv orig stack stack'' \<longrightarrow> stack'' = stack'"
+    using reborrow_unique * by auto
+  ultimately show ?thesis by blast
+qed
+
+lemma the_reborrow'_writable:
+  assumes
+    "wf_reborrow stack"
+    "writable orig stack"
+  shows "\<exists>!stack'. reborrow' k deriv orig stack stack'"
+  using assms ex_reborrow'_writable reborrow_unique by auto
+
+lemma the_reborrow'_readable:
+  assumes
+    "wf_reborrow stack"
+    "readable orig stack"
+    "k = SharedReadOnly"
+  shows "\<exists>!stack'. reborrow' k deriv orig stack stack'"
+  using assms ex_reborrow'_readable reborrow_unique by fastforce
+
+lemma reborrow'_hd:
+  assumes "reborrow' k deriv orig stack stack'"
+  shows "k = fst (hd stack') \<and> deriv \<in> snd (hd stack')"
+using assms proof (induction rule: reborrow'.induct, auto)
+qed
+
+lemma wf_reborrow_reborrow':
+  assumes
+    "reborrow' k deriv orig stack stack'"
+    "wf_reborrow stack"
+    "deriv \<notin> collect_tags stack"
+  shows "wf_reborrow stack'"
+using assms proof (induction)
+  case (DerivPop k deriv orig tail stack entry)
+  then show ?case using reborrow'_nonempty_src wf_reborrow_pop' by auto
+qed (auto simp add: ReborrowSRWSRW ReborrowSROSRO)
+
+lemma wf_reborrow_reborrow'_the:
+  assumes
+    "writable orig stack"
+    "wf_reborrow stack"
+    "deriv \<notin> collect_tags stack"
+  shows "wf_reborrow (THE stack'. reborrow' k deriv orig stack stack')"
+  using assms wf_reborrow_reborrow'
+  by (metis reborrow_by_comp the_reborrow'_writable the_reborrow_by_comp the_reborrow_by_comp')
+
+lemma stack_finite_reborrow':
+  assumes
+    "reborrow' k deriv orig stack stack'"
+    "stack_finite stack"
+  shows "stack_finite stack'"
+using assms proof (induction, auto)
+qed
+
+lemma reborrow'_subset:
+  assumes "reborrow' k deriv orig stack stack'"
+  shows "collect_tags stack' \<subseteq> {deriv} \<union> collect_tags stack"
+using assms proof (induction, auto)
+qed
+
+
+lemma writable_reborrow:
+  assumes
+    "reborrow' k deriv orig stack stack'"
+    "wf_reborrow stack"
+    "writable orig stack"
+    "deriv \<notin> collect_tags stack"
+  shows "writable orig stack'"
+using assms proof (induction)
+  case (DerivPop k deriv orig tail stack entry)
+  show ?case
+  proof (rule DerivPop.IH)
+    show "wf_reborrow tail" using DerivPop wf_reborrow_pop' reborrow'_nonempty_src by simp
+  next
+    show "writable orig tail" using DerivPop writable_tl by fastforce
+  next
+    show "deriv \<notin> collect_tags tail" using DerivPop.prems by simp
+  qed
+qed auto
+
+lemma writable_reborrow_the:
+  assumes
+    "wf_reborrow stack"
+    "writable orig stack"
+    "deriv \<notin> collect_tags stack"
+  shows "writable orig (THE stack'. reborrow' k deriv orig stack stack')"
+  using writable_reborrow
+  by (metis assms ex_reborrow'_writable reborrow_by_comp the_reborrow_by_comp')
+
+lemma writable_reborrow_derived:
+  assumes
+    "reborrow' k deriv orig stack stack'"
+    "writable orig stack"
+    "wf_reborrow stack"
+    "k = Unique \<or> k = SharedReadWrite"
+  shows "writable deriv stack'"
+using assms proof (induction)
+  case (DerivPop k deriv orig tail stack entry)
+  show ?case
+  proof (rule DerivPop.IH)
+    show "wf_reborrow tail" using DerivPop wf_reborrow_pop' reborrow'_nonempty_src by simp
+  next
+    show "writable orig tail" using DerivPop writable_tl by fastforce
+  next
+    show "k = Unique \<or> k = SharedReadWrite" using DerivPop.prems by simp
+  qed
+qed auto
+
+lemma writable_reborrow_derived_the:
+  assumes
+    "writable orig stack"
+    "wf_reborrow stack"
+    "k = Unique \<or> k = SharedReadWrite"
+  shows "writable deriv (THE stack'. reborrow' k deriv orig stack stack')"
+  using writable_reborrow_derived
+  by (metis assms ex_reborrow'_writable reborrow_by_comp the_reborrow_by_comp')
+
+end
